variations on typed fold for lambda
- The implementations differ a lot in terms of speed.
- They don't have proofs, but essentially soundness will require
  that they are called on well-typed terms.

examples/ExprDemo.v
@@ -1,9 +1,9 @@
-Require Import BinPos.
+Require Import Coq.PArith.BinPos.
 Require Import ExtLib.Data.List.
 Require Import ExtLib.Data.HList.
 Require Import MirrorCore.Ext.Types.
 Require Import MirrorCore.Ext.Expr.
-Require Import MirrorCore.Ext.SymEnv.
+Require Import MirrorCore.SymPolyEnv.
 
 (** Demo **)
 Section Demo.
@@ -17,9 +17,9 @@ Section Demo.
 
   Let tyNat := tyType 1.
 
-  Definition funcs' : functions types'.
+  Definition funcs' : functions typD.
   refine (from_list (
-          F types' 0
+          F typD 0
              (tyArr tyNat (tyArr tyNat tyNat))
              plus ::
           F _ 1
@@ -31,17 +31,20 @@ Section Demo.
           F _ 1
              (tyArr (tyVar 0) (tyArr (tyVar 0) tyProp))
              (fun T : Type => @eq T) ::
-          F types' 0 (tyType 1) 0 ::
+          F typD 0 (tyType 1) 0 ::
           nil)).
   Defined.
 
-  Definition App_list (f : expr func) (args : list (expr func)) : expr func :=
+  Definition App_list (f : expr (func typ)) (args : list (expr (func typ)))
+  : expr (func typ) :=
     List.fold_left App args f.
 
   Goal
-    let e := @App_list (Inj (FRef 2%positive (tyType 1 :: nil)))
-                    ((Abs tyNat (@App_list (Inj (FRef 4%positive (tyType 1 :: nil)))
-                                                ((Var 0) :: Inj (FRef 5%positive nil) :: nil))) :: nil) in
+    let e :=
+        @App_list (Inj (FRef 2%positive (tyType 1 :: nil)))
+                  ((Abs tyNat (@App_list (Inj (FRef 4%positive (tyType 1 :: nil)))
+                                         ((Var 0) :: Inj (FRef 5%positive nil) :: nil))) :: nil)
+    in
     match exprD (Expr := Expr_expr (RSym_func funcs')) nil nil e tyProp with
       | None => False
       | Some p => p
