theories/Lambda/ExprD.v
@@ -1,4 +1,31 @@
+Require Import MirrorCore.ExprI.
+Require Import MirrorCore.SymI.
+Require Import MirrorCore.Lambda.TypesI2.
+Require Import MirrorCore.Lambda.ExprCore.
 Require MirrorCore.Lambda.ExprDsimul.
+
+Set Implicit Arguments.
+Set Strict Implicit.
 
 (** Here I need my instance **)
 Export ExprDsimul.ExprDenote.
+
+Section Expr.
+  Context {typ : Type}
+          {typD : list Type -> typ -> Type}
+          {func : Type}.
+  Context {RT : RType typD}
+          {T2 : Typ2 typD PreFun.Fun}
+          {RS : RSym typD func}.
+
+  Instance Expr_expr : @Expr typ typD (@expr typ func) :=
+  { exprD' := fun tus tvs e t =>
+                @exprD' typ typD _ _ _ _ nil tus tvs t e
+  ; wf_Expr_acc := @wf_expr_acc typ func
+  }.
+
+  Instance ExprOk_expr (ts : list Type) : ExprOk Expr_expr.
+  (** TODO(gmalecha): this proof should be here **)
+  Admitted.
+
+End Expr.
