theories/Lambda/TypedFold.v
@@ -1,0 +1,49 @@
+Require MirrorCore.Lambda.TypedFoldLazy.
+
+Set Implicit Arguments.
+Set Strict Implicit.
+
+Definition typed_mfold_lazy
+           (typ : Type) (typD : list Type -> typ -> Type) (func : Type)
+           (_ : SymI.RSym typD func)
+           (_ : TypesI2.Typ2 typD PreFun.Fun)
+           (ts : list Type)
+           (T : Type)
+       (do_var : ExprCore.var -> typ -> TypedFoldLazy.Lazy T)
+       (do_uvar : ExprCore.uvar -> typ -> TypedFoldLazy.Lazy T)
+       (do_inj : func -> typ -> TypedFoldLazy.Lazy T)
+       (do_app : list typ -> list typ -> typ -> typ ->
+                 TypedFoldLazy.Lazy T -> TypedFoldLazy.Lazy T -> TypedFoldLazy.Lazy T)
+       (do_abs : list typ -> list typ -> typ -> typ ->
+                 TypedFoldLazy.Lazy T -> TypedFoldLazy.Lazy T)
+       (tus tvs : list typ) (t : typ) (e : ExprCore.expr typ func)
+: option T :=
+  @TypedFoldLazy.typed_mfold_cpsL typ typD func _ _ ts T
+                                  do_var do_uvar do_inj do_app do_abs
+                                  (option T) tus tvs t e
+                                  (fun x => x tt)
+                                  None.
+
+Definition typed_mfold_infer_lazy
+           (typ : Type) (typD : list Type -> typ -> Type) (func : Type)
+           (_ : SymI.RSym typD func)
+           (_ : TypesI2.Typ2 typD PreFun.Fun)
+           (ts : list Type)
+           (T : Type)
+       (do_var : ExprCore.var -> typ -> TypedFoldLazy.Lazy T)
+       (do_uvar : ExprCore.uvar -> typ -> TypedFoldLazy.Lazy T)
+       (do_inj : func -> typ -> TypedFoldLazy.Lazy T)
+       (do_app : list typ -> list typ -> typ -> typ ->
+                 TypedFoldLazy.Lazy T -> TypedFoldLazy.Lazy T -> TypedFoldLazy.Lazy T)
+       (do_abs : list typ -> list typ -> typ -> typ ->
+                 TypedFoldLazy.Lazy T -> TypedFoldLazy.Lazy T)
+       (tus tvs : list typ) (e : ExprCore.expr typ func)
+: option (typ * T) :=
+  @TypedFoldLazy.typed_mfold_infer_cpsL typ typD func _ _ ts T
+                                  do_var do_uvar do_inj do_app do_abs
+                                  (option (typ * T)) tus tvs e
+                                  (fun t x => match x tt with
+                                                | None => None
+                                                | Some val => Some (t,val)
+                                              end)
+                                  None.
